Define and prove the soundness of more transformations, including the commutativity of (EJoin LikeBag) and filter pushdown under bag semantics

fiat2/src/fiat2/RelTransf.v
@@ -4,6 +4,270 @@ From Stdlib Require Import List String ZArith Permutation.
 
 Open Scope string_scope.
 
+Definition swap_if_nil_head (e : expr) :=
+  (* Swap potential filter constructs to facilitate swap_flatmap_if_head *)
+  match e with
+  | EIf p1 (EIf p2 e1 (EAtom (ANil t))) (EAtom (ANil _)) =>
+
+      EIf p2 (EIf p1 e1 (EAtom (ANil t))) (EAtom (ANil t))
+  | _ => e
+  end.
+
+Section WithMap.
+  Context {tenv: map.map string type} {tenv_ok: map.ok tenv}.
+  Context {width: Z} {word: word.word width} {word_ok: word.ok word}.
+  Notation value := (value (word:=word)).
+  Context {locals: map.map string value} {locals_ok: map.ok locals}.
+
+  Lemma swap_if_nil_head_preserve_ty : forall Gstore, preserve_ty Gstore swap_if_nil_head.
+  Proof.
+    unfold preserve_ty. intros Gstore e t Genv H_Gstore H_Genv H.
+    repeat destruct_subexpr.
+    simpl. repeat (case_match; auto).
+    repeat invert_type_of_clear.
+    repeat constructor; auto.
+  Qed.
+
+  Lemma swap_if_nil_head_preserve_sem : forall Gstore (store : locals),
+      preserve_sem Gstore store swap_if_nil_head.
+  Proof.
+    unfold preserve_sem. intros Gstore store e t Genv env H_Gstore H_Genv H H_str H_env.
+    repeat destruct_subexpr. simpl. repeat (case_match; auto; []). simpl.
+    repeat invert_type_of_clear.
+    apply_type_sound e1; invert_type_of_value_clear.
+    apply_type_sound e2_1; invert_type_of_value_clear.
+    repeat case_match; reflexivity.
+  Qed.
+
+  Lemma swap_if_nil_head_sound : expr_transf_sound (locals:=locals) swap_if_nil_head.
+  Proof.
+    unfold expr_transf_sound; split; intros.
+    1: apply swap_if_nil_head_preserve_ty; auto.
+    eapply swap_if_nil_head_preserve_sem; resolve_locals_wf; eauto.
+  Qed.
+End WithMap.
+
+Definition merge_if_head (e : expr) :=
+  match e with
+  | EIf p1 (EIf p2 e1 (EAtom (ANil t))) (EAtom (ANil _)) =>
+      EIf (EBinop OAnd p1 p2) e1 (EAtom (ANil t))
+  | _ => e
+  end.
+
+Section WithMap.
+  Context {tenv: map.map string type} {tenv_ok: map.ok tenv}.
+  Context {width: Z} {word: word.word width} {word_ok: word.ok word}.
+  Notation value := (value (word:=word)).
+  Context {locals: map.map string value} {locals_ok: map.ok locals}.
+
+  Lemma merge_if_head_preserve_ty : forall Gstore, preserve_ty Gstore merge_if_head.
+  Proof.
+    unfold preserve_ty. intros Gstore e t Genv H_Gstore H_Genv H.
+    repeat destruct_subexpr.
+    simpl. repeat (case_match; auto).
+    repeat invert_type_of_clear.
+    repeat econstructor; eauto.
+  Qed.
+
+  Lemma merge_if_head_preserve_sem : forall Gstore (store : locals),
+      preserve_sem Gstore store merge_if_head.
+  Proof.
+    unfold preserve_sem. intros Gstore store e t Genv env H_Gstore H_Genv H H_str H_env.
+    repeat destruct_subexpr. simpl. repeat (case_match; auto; []). simpl.
+    repeat invert_type_of_clear.
+    apply_type_sound e1; invert_type_of_value_clear.
+    apply_type_sound e2_1; invert_type_of_value_clear.
+    cbn; destruct b, b0; reflexivity.
+  Qed.
+
+  Lemma merge_if_head_sound : expr_transf_sound (locals:=locals) merge_if_head.
+  Proof.
+    unfold expr_transf_sound; split; intros.
+    1: apply merge_if_head_preserve_ty; auto.
+    eapply merge_if_head_preserve_sem; resolve_locals_wf; eauto.
+  Qed.
+End WithMap.
+
+Definition swap_flatmap_if_head (e : expr) :=
+  (* Push potential filter construct closer to the relevant table *)
+  match e with
+  | EFlatmap LikeList e1 x1 (EIf p e2 (EAtom (ANil t))) =>
+      if free_immut_in x1 p then e
+      else EIf p (EFlatmap LikeList e1 x1 e2) (EAtom (ANil t))
+  | _ => e
+  end.
+
+Section WithMap.
+  Context {tenv: map.map string type} {tenv_ok: map.ok tenv}.
+  Context {width: Z} {word: word.word width} {word_ok: word.ok word}.
+  Notation value := (value (word:=word)).
+  Context {locals: map.map string value} {locals_ok: map.ok locals}.
+
+  Lemma swap_flatmap_if_head_preserve_ty : forall Gstore, preserve_ty Gstore swap_flatmap_if_head.
+  Proof.
+    unfold preserve_ty. intros Gstore e t Genv H_Gstore H_Genv H.
+    repeat destruct_subexpr.
+    simpl. repeat (case_match; auto).
+    repeat invert_type_of_clear.
+    repeat econstructor; eauto using not_free_immut_put_ty.
+  Qed.
+
+  Lemma swap_flatmap_if_head_preserve_sem : forall Gstore (store : locals),
+      preserve_sem Gstore store swap_flatmap_if_head.
+  Proof.
+    unfold preserve_sem. intros Gstore store e t Genv env H_Gstore H_Genv H H_str H_env.
+    repeat destruct_subexpr. simpl. repeat (case_match; auto; []). simpl.
+    repeat invert_type_of_clear.
+    apply_type_sound e1; invert_type_of_value_clear.
+    lazymatch goal with
+      H: VList _ = _ |- _ => clear H
+    end.
+    lazymatch goal with
+      H: type_of _ (map.put _ _ _) _ TBool |- _ =>
+        apply not_free_immut_put_ty in H
+    end; trivial.
+    apply_type_sound e2_1; invert_type_of_value_clear.
+    case_match; f_equal; subst.
+    2:{ erewrite flat_map_eq.
+        2:{ rewrite Forall_forall; intros.
+            rewrite <- not_free_immut_put_sem; trivial.
+            repeat rewrite_r_to_l.
+            repeat rewrite_l_to_r.
+            instantiate (1:=fun _ => nil).
+            reflexivity. }
+        clear. induction l; auto. }
+    apply flat_map_eq.
+    rewrite Forall_forall; intros.
+    rewrite <- (not_free_immut_put_sem e2_1); trivial.
+    repeat rewrite_r_to_l. reflexivity.
+  Qed.
+
+  Lemma swap_flatmap_if_head_sound : expr_transf_sound (locals:=locals) swap_flatmap_if_head.
+  Proof.
+    unfold expr_transf_sound; split; intros.
+    1: apply swap_flatmap_if_head_preserve_ty; auto.
+    eapply swap_flatmap_if_head_preserve_sem; resolve_locals_wf; eauto.
+  Qed.
+End WithMap.
+
+Definition singleton (e : expr) :=
+  EBinop OCons e (EAtom (ANil None)).
+
+Lemma flat_map__flat_map : forall A B C (f : B -> list C) (g : A -> list B) l,
+    flat_map f (flat_map g l) = flat_map (fun x => flat_map f (g x)) l.
+Proof.
+  induction l; auto. cbn.
+  rewrite flat_map_app. congruence.
+Qed.
+
+Definition if_nil_into_flatmap_head (e : expr) :=
+  (* Expose filter construct *)
+  match e with
+  | EFlatmap LikeList e1 x (EIf p e2 (EAtom (ANil t))) =>
+      EFlatmap LikeList (EFlatmap LikeList e1 x (EIf p (singleton (EVar x)) (EAtom (ANil None)))) x e2
+  | _ => e
+  end.
+
+Section WithMap.
+  Context {tenv: map.map string type} {tenv_ok: map.ok tenv}.
+  Context {width: Z} {word: word.word width} {word_ok: word.ok word}.
+  Notation value := (value (word:=word)).
+  Context {locals: map.map string value} {locals_ok: map.ok locals}.
+
+  Lemma if_nil_into_flatmap_head_preserve_ty : forall Gstore, preserve_ty Gstore if_nil_into_flatmap_head.
+  Proof.
+    unfold preserve_ty. intros Gstore e t Genv H_Gstore H_Genv H.
+    repeat destruct_subexpr.
+    simpl. repeat (case_match; auto).
+    repeat invert_type_of_clear.
+    repeat (econstructor ; eauto with fiat2_hints).
+    rewrite_map_get_put_goal. reflexivity.
+  Qed.
+
+  Lemma if_nil_into_flatmap_head_preserve_sem : forall Gstore (store : locals),
+      preserve_sem Gstore store if_nil_into_flatmap_head.
+  Proof.
+    unfold preserve_sem. intros Gstore store e t Genv env H_Gstore H_Genv H H_str H_env.
+    repeat destruct_subexpr. simpl. repeat (case_match; auto; []). simpl.
+    repeat invert_type_of_clear.
+    apply_type_sound e1; invert_type_of_value_clear.
+    lazymatch goal with
+      _: VList _ = ?x, H': ?x = _ |- _ =>
+        rewrite H' in *; clear H'
+    end. do_injection; clear_refl.
+    f_equal; subst.
+    rewrite flat_map__flat_map.
+    apply flat_map_eq.
+    rewrite Forall_forall; intros.
+    apply_Forall_In.
+    apply_type_sound e2_1; eauto with fiat2_hints. invert_type_of_value_clear.
+    unfold get_local. rewrite_map_get_put_goal.
+    case_match; cbn; auto.
+    rewrite app_nil_r. reflexivity.
+  Qed.
+
+  Lemma if_nil_into_flatmap_head_sound : expr_transf_sound (locals:=locals) if_nil_into_flatmap_head.
+  Proof.
+    unfold expr_transf_sound; split; intros.
+    1: apply if_nil_into_flatmap_head_preserve_ty; auto.
+    eapply if_nil_into_flatmap_head_preserve_sem; resolve_locals_wf; eauto.
+  Qed.
+End WithMap.
+
+Definition join_to_flatmap_filter_head (e : expr) :=
+  match e with
+  | EJoin LikeList e1 e2 x1 x2 p e3 =>
+      if free_immut_in x1 e2 then e
+      else EFlatmap LikeList e1 x1
+             (EFlatmap LikeList (EFilter LikeList e2 x2 p) x2
+                (EBinop OCons e3 (EAtom (ANil None))))
+  | _ => e
+  end.
+
+Section WithMap.
+  Context {tenv: map.map string type} {tenv_ok: map.ok tenv}.
+  Context {width: Z} {word: word.word width} {word_ok: word.ok word}.
+  Notation value := (value (word:=word)).
+  Context {locals: map.map string value} {locals_ok: map.ok locals}.
+
+  Lemma join_to_flatmap_filter_head_preserve_ty : forall Gstore, preserve_ty Gstore join_to_flatmap_filter_head.
+  Proof.
+    unfold preserve_ty. intros Gstore e t Genv H_Gstore H_Genv H.
+    repeat destruct_subexpr.
+    simpl. repeat (case_match; auto).
+    repeat invert_type_of_clear.
+    repeat econstructor; eauto using not_free_immut_put_ty2.
+    eapply type_of__type_wf. 3: eassumption.
+    1: eauto with fiat2_hints.
+    repeat apply tenv_wf_step; eauto with fiat2_hints.
+  Qed.
+
+  Lemma join_to_flatmap_filter_head_preserve_sem : forall Gstore (store : locals),
+      preserve_sem Gstore store join_to_flatmap_filter_head.
+  Proof.
+    unfold preserve_sem. intros Gstore store e t Genv env H_Gstore H_Genv H H_str H_env.
+    repeat destruct_subexpr. simpl. repeat (case_match; auto; []). simpl.
+    repeat invert_type_of_clear.
+    apply_type_sound e1; invert_type_of_value_clear.
+    lazymatch goal with
+      H: VList _ = _ |- _ => clear H
+    end.
+    apply_type_sound e2; invert_type_of_value_clear.
+    f_equal; subst.
+    apply flat_map_eq.
+    rewrite Forall_forall; intros.
+    rewrite <- (not_free_immut_put_sem e2); trivial.
+    repeat rewrite_r_to_l. reflexivity.
+  Qed.
+
+  Lemma join_to_flatmap_filter_head_sound : expr_transf_sound (locals:=locals) join_to_flatmap_filter_head.
+  Proof.
+    unfold expr_transf_sound; split; intros.
+    1: apply join_to_flatmap_filter_head_preserve_ty; auto.
+    eapply join_to_flatmap_filter_head_preserve_sem; resolve_locals_wf; eauto.
+  Qed.
+End WithMap.
+
 Definition to_filter_head (e : expr) :=
   match e with
   | EFlatmap LikeList e' x
@@ -196,6 +460,119 @@ Section WithMap.
   Qed.
 End WithMap.
 
+Definition filter_pushdown_likebag_head (e : expr) :=
+  match e with
+  | EJoin LikeBag tbl1 tbl2 r1 r2 (EBinop OAnd p1 p) r =>
+      if free_immut_in r2 p1
+      then e
+      else EJoin LikeBag (EFilter LikeBag tbl1 r1 p1) tbl2 r1 r2 p r
+  | _ => e
+  end.
+
+Section WithMap.
+  Context {tenv: map.map string type} {tenv_ok: map.ok tenv}.
+  Context {width: Z} {word: word.word width} {word_ok: word.ok word}.
+  Notation value := (value (word:=word)).
+  Context {locals: map.map string value} {locals_ok: map.ok locals}.
+
+  Lemma filter_pushdown_likebag_head_preserve_ty : forall Gstore,
+      preserve_ty Gstore filter_pushdown_likebag_head.
+  Proof.
+    unfold preserve_ty. intros Gstore e t Genv H_Gstore H_Genv H.
+    repeat destruct_subexpr.
+    simpl. repeat (case_match; auto).
+    repeat invert_type_of_clear. invert_type_of_op.
+    econstructor; eauto. constructor; auto.
+    eapply not_free_immut_put_ty; eauto.
+  Qed.
+
+  Lemma filter_repeat_true : forall A f (v : A) n,
+      f v = true -> filter f (repeat v n) = repeat v n.
+  Proof.
+    induction n; cbn; auto.
+    intros. repeat rewrite_l_to_r.
+    intuition idtac. congruence.
+  Qed.
+
+  Lemma filter_repeat_false : forall A f (v : A) n,
+      f v = false -> filter f (repeat v n) = nil.
+  Proof.
+    induction n; cbn; auto.
+    intros. repeat rewrite_l_to_r.
+    intuition idtac.
+  Qed.
+
+  Lemma bag_to_list_filter_fst : forall (f : value -> bool) l,
+      bag_to_list (filter (fun v => f (fst v)) l) =
+        filter f (bag_to_list l).
+  Proof.
+    induction l; cbn; auto. destruct a; cbn.
+    case_match; cbn; rewrite IHl, filter_app.
+    1: rewrite filter_repeat_true; auto.
+    1: rewrite filter_repeat_false; auto.
+  Qed.
+
+  Lemma filter_pushdown_likebag_head_preserve_sem : forall Gstore (store : locals),
+      preserve_sem Gstore store filter_pushdown_likebag_head.
+  Proof.
+    unfold preserve_sem. intros Gstore store e t Genv env H_Gstore H_Genv H H_str H_env.
+    repeat destruct_subexpr. simpl.
+    repeat (case_match; auto; []). simpl.
+    repeat invert_type_of_clear.
+    invert_type_of_op_clear.
+    apply_type_sound e1; invert_type_of_value_clear.
+    apply_type_sound e2; invert_type_of_value_clear.
+    do 2 f_equal.
+    erewrite bag_to_list_filter_fst with
+      (f := fun v : value =>
+              match
+                interp_expr store (map.put env x v) e3_1
+              with
+              | VBool b => b
+              | _ => false
+              end).
+    rewrite flat_map_filter.
+    apply flat_map_eq.
+    rewrite Forall_forall; intros ? H_in.
+    apply bag_to_list_incl, In_fst in H_in.
+    destruct_exists; intuition idtac.
+    apply_Forall_In.
+    lazymatch goal with
+      H: type_of _ _ e3_1 _ |- _ =>
+        apply not_free_immut_put_ty in H
+      end; auto.
+    apply_type_sound e3_1;
+      eauto with fiat2_hints.
+    invert_type_of_value_clear; rewrite_expr_value.
+    case_match.
+    1:{ f_equal. apply filter_ext_in; intros ? H_in.
+    apply bag_to_list_incl, In_fst in H_in.
+    destruct_exists; intuition idtac.
+    apply_Forall_In.
+    rewrite <- not_free_immut_put_sem with (e:=e3_1); auto.
+    rewrite_expr_value; cbn.
+    case_match; auto. }
+    1:{ symmetry; apply List.map_nil.
+        apply List.filter_nil; intros ? H_in.
+    apply bag_to_list_incl, In_fst in H_in.
+    destruct_exists; intuition idtac.
+    apply_Forall_In.
+    rewrite <- not_free_immut_put_sem with (e:=e3_1); auto.
+    rewrite_expr_value; cbn.
+    apply_type_sound e3_2; eauto with fiat2_hints.
+    2: repeat apply tenv_wf_step; eauto with fiat2_hints.
+    invert_type_of_value_clear.
+    rewrite_expr_value; reflexivity. }
+  Qed.
+
+  Lemma filter_pushdown_likebag_head_sound : expr_transf_sound (locals:=locals) filter_pushdown_likebag_head.
+  Proof.
+    unfold expr_transf_sound; split; intros.
+    1: apply filter_pushdown_likebag_head_preserve_ty; auto.
+    eapply filter_pushdown_likebag_head_preserve_sem; resolve_locals_wf; eauto.
+  Qed.
+End WithMap.
+
 Definition to_proj_head (e : expr) :=
   match e with
   | EFlatmap LikeList e x
@@ -233,6 +610,159 @@ Section WithMap.
     unfold expr_transf_sound; split; intros.
     1: apply to_proj_head_preserve_ty; auto.
     eapply to_proj_head_preserve_sem; resolve_locals_wf; eauto.
+  Qed.
+End WithMap.
+
+Definition swap_join_likebag_head (e : expr) :=
+  match e with
+  | EJoin LikeBag e1 e2 x1 x2 p e3 =>
+      if String.eqb x1 x2 then e
+      else EJoin LikeBag e2 e1 x2 x1 p e3
+  | _ => e
+  end.
+
+Section WithMap.
+  Context {tenv: map.map string type} {tenv_ok: map.ok tenv}.
+  Context {width: Z} {word: word.word width} {word_ok: word.ok word}.
+  Notation value := (value (word:=word)).
+  Context {locals: map.map string value} {locals_ok: map.ok locals}.
+
+  Lemma swap_join_likebag_head_preserve_ty : forall Gstore, preserve_ty Gstore swap_join_likebag_head.
+  Proof.
+    unfold preserve_ty. intros Gstore e t Genv H_Gstore H_Genv H.
+    repeat destruct_subexpr.
+    simpl. repeat (case_match; auto).
+    repeat invert_type_of_clear.
+    rewrite String.eqb_neq in *.
+    econstructor; eauto.
+    all: rewrite Properties.map.put_put_diff; auto.
+  Qed.
+
+  Lemma bag_insert_comm : forall (x y : value) l,
+      bag_insert x (bag_insert y l) = bag_insert y (bag_insert x l).
+  Proof.
+    induction l; cbn; unfold value_ltb, value_eqb.
+    1:{ case_match.
+        all: try lazymatch goal with
+                 E: _ = Eq |- _ =>
+                   apply value_compare_Eq_eq in E;
+                   subst;
+                   rewrite value_compare_refl
+               end.
+        all: repeat (rewrite value_compare_antisym; rewrite_l_to_r); cbn; auto. }
+    1:{ repeat case_match; cbn.
+        all: repeat lazymatch goal with
+                 E: _ = Eq |- _ =>
+                   apply value_compare_Eq_eq in E;
+                   subst
+               end; trivial.
+        all: unfold value_ltb, value_eqb;
+          try rewrite value_compare_refl;
+          repeat rewrite_l_to_r; auto.
+        all: repeat (rewrite value_compare_antisym; rewrite_l_to_r); cbn; auto.
+        all: case_match;
+          try lazymatch goal with
+              E: _ = Eq |- _ =>
+                apply value_compare_Eq_eq in E;
+                subst
+            end;
+          try rewrite value_compare_refl; auto.
+        all: repeat (rewrite value_compare_antisym; rewrite_l_to_r); cbn; auto.
+        all: repeat rewrite_l_to_r; try discriminate.
+        all: lazymatch goal with
+            H1: value_compare ?a ?b = Lt,
+              H2: value_compare ?b ?c = Lt |- _ =>
+              eapply (value_compare_trans _ _ _ H1) in H2
+          end; rewrite_l_to_r; discriminate. }
+  Qed.
+
+  Lemma Permutation_list_to_bag_eq : forall (l l' : list value),
+      Permutation l l' ->
+      list_to_bag l = list_to_bag l'.
+  Proof.
+    induction 1; cbn; try congruence.
+    apply bag_insert_comm.
+  Qed.
+
+  Lemma Permutation_flat_map_app : forall A B (f : A -> list B) g l,
+      Permutation
+        (flat_map (fun x => (f x ++ g x)%list) l)
+        (flat_map f l ++ flat_map g l).
+  Proof.
+    induction l; cbn; auto.
+    rewrite IHl.
+    rewrite <- !app_assoc.
+    apply Permutation_app_head.
+    rewrite !app_assoc.
+    apply Permutation_app_tail.
+    apply Permutation_app_comm.
+  Qed.
+
+  Lemma Permutation_flat_map_comm : forall A B C (f : A -> B -> list C) l l',
+      Permutation
+        (flat_map (fun x => flat_map (fun y => f x y) l) l')
+        (flat_map (fun y => flat_map (fun x => f x y) l') l).
+  Proof.
+    induction l; cbn.
+    1: induction l'; auto.
+    intros.
+    rewrite Permutation_flat_map_app, IHl.
+    auto.
+  Qed.
+
+  Lemma map_filter__flat_map : forall A B (f : A -> B) g l,
+      map f (filter g l) = flat_map (fun x => if g x then f x :: nil else nil) l.
+  Proof.
+    induction l; cbn; auto.
+    case_match; cbn; congruence.
+  Qed.
+
+  Lemma swap_join_likebag_head_preserve_sem : forall Gstore (store : locals),
+      preserve_sem Gstore store swap_join_likebag_head.
+  Proof.
+    unfold preserve_sem. intros Gstore store e t Genv env H_Gstore H_Genv H H_str H_env.
+    repeat destruct_subexpr. simpl.
+    repeat (case_match; auto; []). simpl.
+    rewrite String.eqb_neq in *.
+    repeat invert_type_of_clear.
+    apply_type_sound e1; invert_type_of_value_clear.
+    apply_type_sound e2; invert_type_of_value_clear.
+    repeat lazymatch goal with
+      H: VBag _ = _ |- _ => clear H
+           end.
+    f_equal.
+    apply Permutation_list_to_bag_eq.
+    erewrite flat_map_eq.
+    (* swap the order of map.put *)
+    2:{ rewrite Forall_forall; intros ? H_in.
+        apply bag_to_list_incl, In_fst in H_in.
+        destruct_exists. destruct_and.
+        apply_Forall_In.
+        erewrite filter_ext_in.
+        2:{ intros ? H_in.
+            apply bag_to_list_incl, In_fst in H_in.
+            destruct_exists. destruct_and.
+            rewrite Properties.map.put_put_diff; auto.
+            reflexivity. }
+        erewrite map_ext_in.
+        2:{ intros.
+            rewrite Properties.map.put_put_diff; auto.
+            reflexivity. }
+        reflexivity. }
+    erewrite flat_map_eq.
+    2:{  rewrite Forall_forall; intros.
+         rewrite map_filter__flat_map . reflexivity. }
+    erewrite flat_map_eq with (l:=bag_to_list l).
+    2:{  rewrite Forall_forall; intros.
+         rewrite map_filter__flat_map . reflexivity. }
+    apply Permutation_flat_map_comm.
+  Qed.
+
+  Lemma swap_join_likebag_head_sound : expr_transf_sound (locals:=locals) swap_join_likebag_head.
+  Proof.
+    unfold expr_transf_sound; split; intros.
+    1: apply swap_join_likebag_head_preserve_ty; auto.
+    eapply swap_join_likebag_head_preserve_sem; resolve_locals_wf; eauto.
   Qed.
 End WithMap.
 
